\begin{frame}{\(\Im w(z)\) и \(\Re w(z)\)}
	Для дальнейшего изучения отображения найдем \( \Im(w(z)) \) и \( \Re(w(z)) \).
	Пусть \( z = u + i v \). Тогда:

	\begin{align*}
		w(z) & = w(u + iv) = 1 - \frac{2}{(u + 1) + iv} = 1 - \frac{2((u + 1) - iv)}{((u+1)+iv)((u+1)-iv)} = \\
		     & = 1 - \frac{2(u + 1 - iv)}{(u+1)^2 + v^2} = 1 - \frac{2u + 2 - 2iv}{u^2 + 2u + v^2 + 1} =     \\
		     & = 1 - \frac{2u+2}{u^2+2u+v^2+1} - i\frac{2v}{u^2+2u+v^2+1} =                                  \\
		     & = \frac{u^2 +v^2 - 1}{u^2+2u+v^2+1} - i \frac{2v}{u^2+2u+v^2+1}
	\end{align*}

	Значит \( \Re(w(z)) = \frac{u^2+v^2-1}{u^2+2u+v^2+1} \), \( \Im(w(z)) = - \frac{2v}{u^2+2u+v^2+1} \)
\end{frame}
